Trying things

GDS_Language.v
@@ -168,21 +168,22 @@ Fixpoint runStmt (fuel: nat) (vg1: valuation) (vl1: valuation) (st: stmt) (vg2: 
         | assignCallMethodStmt ret method_name args =>
             match vg1 $? method_name with 
             | Some (methodAss name_args found_ret found_body) => 
-                exists vlmid,
+                exists vlmid vgmid,
                 runStmt fuel' vg1 
                 (fold_left 
                     (fun (acc: valuation) (arg_argname: expr * string) => 
                         (acc $+ ((snd arg_argname), varAss (interp2 (fst arg_argname) vg1 vl1)))
                     ) 
                     (combine args name_args) ($0)) 
-                found_body vg2 vlmid
+                found_body vgmid vlmid
                 /\ match ret, found_ret with
                     | Some s_ret, Some s_found_ret => 
                         (exists r, interp (Var s_found_ret) vlmid = r 
                         /\ 
-                        ((runStmt fuel' vg1 vl1 (assignmentStmt s_ret (Const r)) vg2 vl2) (* if already defined (locally or globally), reassign to new value r *)
+                        ((runStmt fuel' vgmid vl1 (assignmentStmt s_ret (Const r)) vg2 vl2) (* if already defined (locally or globally), reassign to new value r *)
                         \/
-                        vl1 $? s_ret = None /\ vg1 $? s_ret = None /\ (vl2 = vl1 $+ (s_ret, varAss r)))) (* otw, new val *)
+                        vl1 $? s_ret = None /\ vgmid $? s_ret = None /\ (vl2 = vl1 $+ (s_ret, varAss r) (* otw, new val *)
+                        )))
                     | Some _, None => False
                     | None, _ => vl2 = vlmid
                     end
